projection/proofs/payload_closureProofScript.sml
@@ -1,0 +1,224 @@
+open preamble payloadSemTheory payloadLangTheory choreoUtilsTheory payload_closureTheory payloadPropsTheory;
+open ConseqConv;
+
+val _ = new_theory "payload_closureProof";
+
+Definition no_undefined_writes_def:
+  no_undefined_writes n =
+  EVERY (λ(p,s,e). set(written_var_names_endpoint e) ⊆ FDOM s.bindings) (endpoints n)
+End
+
+Theorem no_undefined_writes_NPar:
+  no_undefined_writes (NPar n1 n2) = (no_undefined_writes n1 ∧ no_undefined_writes n2)
+Proof
+  rw[no_undefined_writes_def,endpoints_def]
+QED
+
+Theorem fix_network_NPar:
+  fix_network (NPar n1 n2) = (fix_network n1 ∧ fix_network n2)
+Proof
+  rw[fix_network_def,endpoints_def]
+QED
+
+Theorem compile_network_preservation_send:
+  ∀p1 p2 conf p3 d p4.
+    conf.payload_size > 0
+    ∧ trans conf p1 (LSend p3 d p4) p2
+    ⇒ trans conf (compile_network_alt p1) (LSend p3 d p4) (compile_network_alt p2)
+Proof
+  Induct_on ‘p1’ >>
+  rw[Once trans_cases,no_undefined_writes_NPar,compile_network_alt_def] >>
+  rw[compile_network_alt_def] >>
+  TRY(rename1 ‘NPar’ >> rw[Once trans_cases] >> NO_TAC) >>
+  fs[no_undefined_writes_def,endpoints_def] >>
+  simp[compile_endpoint_def] >>
+  rw[Once trans_cases,PULL_EXISTS] >>
+  rw[flookup_update_list_some,ALOOKUP_MAP,written_var_names_endpoint_def,ALOOKUP_NONE,MEM_MAP,MEM_FILTER,MEM_nub',PULL_EXISTS,FDOM_FLOOKUP,LEFT_AND_OVER_OR,RIGHT_AND_OVER_OR,EXISTS_OR_THM]
+QED
+
+Theorem compile_network_preservation_receive:
+  ∀p1 p2 conf p3 d p4.
+    conf.payload_size > 0
+    ∧ trans conf p1 (LReceive p3 d p4) p2
+    ⇒ trans conf (compile_network_alt p1) (LReceive p3 d p4) (compile_network_alt p2)
+Proof
+  Induct_on ‘p1’ >>
+  rw[Once trans_cases,no_undefined_writes_NPar,compile_network_alt_def] >>
+  rw[compile_network_alt_def] >>
+  TRY(rename1 ‘NPar’ >> rw[Once trans_cases] >> NO_TAC) >>
+  fs[no_undefined_writes_def,endpoints_def] >>
+  simp[compile_endpoint_def] >>
+  rw[Once trans_cases,PULL_EXISTS] >>
+  rw[flookup_update_list_some,ALOOKUP_MAP,written_var_names_endpoint_def,ALOOKUP_NONE,MEM_MAP,MEM_FILTER,MEM_nub',PULL_EXISTS,FDOM_FLOOKUP,LEFT_AND_OVER_OR,RIGHT_AND_OVER_OR,EXISTS_OR_THM]
+QED
+
+(* TODO: Figure out a useful relation to put here *)
+Inductive compile_rel:
+  ∀x. compile_rel x (x:network)
+End
+
+Theorem compile_rel_refl:
+  compile_rel x x
+Proof
+  cheat
+QED
+
+Theorem compile_rel_reflI:
+  ∀x y. x = y ⇒ compile_rel x y
+Proof
+  simp[compile_rel_refl]
+QED
+
+Theorem ALOOKUP_MAP_CONST_EQ:
+  ALOOKUP(MAP (λx. (x,k)) l) x =
+  if MEM x l then SOME k else NONE
+Proof
+  Induct_on ‘l’ >> rw[] >> fs[]
+QED
+
+Theorem compile_network_preservation_trans:
+  ∀p1 p2 conf.
+    conf.payload_size > 0
+(*    ∧ no_undefined_writes p1*)
+    ∧ fix_network p1
+    ∧ reduction conf p1 p2
+    ⇒ ∃p3. (reduction conf)^* (compile_network_alt p1) p3 ∧
+             compile_rel p3 (compile_network_alt p2)
+Proof
+  rpt strip_tac
+  >> qhdtm_x_assum ‘reduction’ (fn thm => rpt(pop_assum mp_tac) >> assume_tac  thm)
+  >> fs[payloadSemTheory.reduction_def]
+  >> qmatch_asmsub_abbrev_tac `trans _ _ alpha _`
+  >> pop_assum (mp_tac o PURE_ONCE_REWRITE_RULE [markerTheory.Abbrev_def])
+  >> pop_assum mp_tac
+  >> MAP_EVERY qid_spec_tac [`p2`,`alpha`,`p1`,‘conf’]
+  >> ho_match_mp_tac payloadSemTheory.trans_strongind
+  >> rpt strip_tac >> fs[] >> rveq
+  >- ((* trans_com_l *)
+      fs[no_undefined_writes_NPar]
+      >> MAP_EVERY (drule_all_then strip_assume_tac)
+                   [compile_network_preservation_send,
+                    compile_network_preservation_receive]
+      >> simp[compile_network_alt_def]
+      >> drule_all_then strip_assume_tac trans_com_l
+      >> fs[GSYM reduction_def]
+      >> drule_then strip_assume_tac RTC_SUBSET
+      >> goal_assum drule
+      >> simp[compile_rel_refl])
+  >- ((* trans_com_r *)
+      fs[no_undefined_writes_NPar]
+      >> MAP_EVERY (drule_all_then strip_assume_tac)
+                   [compile_network_preservation_send,
+                    compile_network_preservation_receive]
+      >> simp[compile_network_alt_def]
+      >> drule_all_then strip_assume_tac trans_com_r
+      >> fs[GSYM reduction_def]
+      >> drule_then strip_assume_tac RTC_SUBSET
+      >> goal_assum drule
+      >> simp[compile_rel_refl])
+  >- ((* trans_dequeue_last_payload *)
+      goal_assum (resolve_then (Pos hd) mp_tac RTC_SUBSET) >>
+      simp[reduction_def] >>
+      simp[compile_network_alt_def,compile_endpoint_def] >>
+      simp[Once trans_cases,RIGHT_AND_OVER_OR,PULL_EXISTS,EXISTS_OR_THM] >>
+      CONSEQ_CONV_TAC(
+        DEPTH_CONSEQ_CONV(
+          CONSEQ_REWRITE_CONV
+          ([],[compile_rel_reflI],[]))) >>
+      fs[state_component_equality,fmap_eq_flookup,FLOOKUP_UPDATE,alookup_distinct_reverse,
+         flookup_fupdate_list,MAP_MAP_o,o_DEF,all_distinct_nub',ALL_DISTINCT_MAP,
+         FILTER_ALL_DISTINCT,ALOOKUP_MAP_CONST_EQ,MEM_FILTER,MEM_nub'] >>
+      csimp[CaseEq "bool",written_var_names_endpoint_def])
+  >- ((* trans_dequeue_intermediate_payload *)
+      goal_assum (resolve_then (Pos hd) mp_tac RTC_SUBSET) >>
+      simp[reduction_def] >>
+      simp[compile_network_alt_def,compile_endpoint_def] >>
+      simp[Once trans_cases,RIGHT_AND_OVER_OR,PULL_EXISTS,EXISTS_OR_THM] >>
+      CONSEQ_CONV_TAC(
+        DEPTH_CONSEQ_CONV(
+          CONSEQ_REWRITE_CONV
+          ([],[compile_rel_reflI],[]))) >>
+      fs[state_component_equality,fmap_eq_flookup,FLOOKUP_UPDATE,alookup_distinct_reverse,
+         flookup_fupdate_list,MAP_MAP_o,o_DEF,all_distinct_nub',ALL_DISTINCT_MAP,
+         FILTER_ALL_DISTINCT,ALOOKUP_MAP_CONST_EQ,MEM_FILTER,MEM_nub'] >>
+      csimp[CaseEq "bool",written_var_names_endpoint_def])
+  >- ((* trans_if_true *)
+      ‘v ∈ FDOM s.bindings’ by simp[FDOM_FLOOKUP] >>
+      goal_assum (resolve_then (Pos hd) mp_tac RTC_SUBSET) >>
+      simp[reduction_def] >>
+      simp[compile_network_alt_def,compile_endpoint_def] >>
+      simp[Once trans_cases,RIGHT_AND_OVER_OR,PULL_EXISTS,EXISTS_OR_THM] >>
+      cheat (* different variables initialised *)
+      (*CONSEQ_CONV_TAC(
+        DEPTH_CONSEQ_CONV(
+          CONSEQ_REWRITE_CONV
+          ([],[compile_rel_reflI],[]))) >>
+      fs[state_component_equality,fmap_eq_flookup,FLOOKUP_UPDATE,alookup_distinct_reverse,
+         flookup_fupdate_list,MAP_MAP_o,o_DEF,all_distinct_nub',ALL_DISTINCT_MAP,
+         FILTER_ALL_DISTINCT,ALOOKUP_MAP_CONST_EQ,MEM_FILTER,MEM_nub'] >>
+      csimp[CaseEq "bool",written_var_names_endpoint_def]*))
+  >- ((* trans_if_false *)
+      ‘v ∈ FDOM s.bindings’ by simp[FDOM_FLOOKUP] >>
+      goal_assum (resolve_then (Pos hd) mp_tac RTC_SUBSET) >>
+      simp[reduction_def] >>
+      simp[compile_network_alt_def,compile_endpoint_def] >>
+      simp[Once trans_cases,RIGHT_AND_OVER_OR,PULL_EXISTS,EXISTS_OR_THM] >>
+      cheat  (* different variables initialised *))
+  >- ((* trans_let *)
+      goal_assum (resolve_then (Pos hd) mp_tac RTC_SUBSET) >>
+      simp[reduction_def] >>
+      simp[compile_network_alt_def,compile_endpoint_def] >>
+      simp[Once trans_cases,RIGHT_AND_OVER_OR,PULL_EXISTS,EXISTS_OR_THM] >>
+      CONSEQ_CONV_TAC(
+        DEPTH_CONSEQ_CONV(
+          CONSEQ_REWRITE_CONV
+          ([],[compile_rel_reflI],[]))) >>
+      fs[state_component_equality,fmap_eq_flookup,FLOOKUP_UPDATE,alookup_distinct_reverse,
+         flookup_fupdate_list,MAP_MAP_o,o_DEF,all_distinct_nub',ALL_DISTINCT_MAP,
+         FILTER_ALL_DISTINCT,ALOOKUP_MAP_CONST_EQ,MEM_FILTER,MEM_nub'] >>
+      csimp[CaseEq "bool",written_var_names_endpoint_def] >>
+      fs[EVERY_MEM,MEM_MAP,PULL_EXISTS,IS_SOME_EXISTS,flookup_update_list_some,
+         MAP_MAP_o,o_DEF,all_distinct_nub',ALL_DISTINCT_MAP,alookup_distinct_reverse,
+         FILTER_ALL_DISTINCT,ALOOKUP_MAP_CONST_EQ,MEM_FILTER,MEM_nub',EXISTS_OR_THM] >>
+      conj_tac >- metis_tac[] >>
+      AP_TERM_TAC >>
+      rw[MAP_EQ_f] >> rw[] >>
+      res_tac >>
+      fs[FDOM_FLOOKUP])
+  >- ((* trans_par_l *)
+      fs[compile_network_alt_def,fix_network_NPar]
+      >> drule_then (fn thm => goal_assum(resolve_then (Pos hd) mp_tac thm)) payloadPropsTheory.reduction_par_l
+      >> cheat (* preserved by parallel *)
+     )
+  >- ((* trans_par_r *)
+      fs[compile_network_alt_def,fix_network_NPar]
+      >> drule_then (fn thm => goal_assum(resolve_then (Pos hd) mp_tac thm)) payloadPropsTheory.reduction_par_r
+      >> cheat (* preserved by parallel *))
+  >- ((* trans_fix *)
+      cheat)
+  >- ((* trans_Letrec *)
+      fs[fix_network_def,endpoints_def,fix_endpoint_def])
+  >- ((* trans_call *)
+      fs[fix_network_def,endpoints_def,fix_endpoint_def])
+QED
+
+Theorem compile_network_preservation:
+  ∀conf p1 p2.
+    conf.payload_size > 0
+    ∧ reduction^* p1 p2 ∧ choice_free_network p1
+    ==> (reduction conf)^* (compile_network conf p1) (compile_network conf p2)
+Proof
+  strip_tac >> simp[GSYM AND_IMP_INTRO,RIGHT_FORALL_IMP_THM]
+  >> strip_tac
+  >> ho_match_mp_tac RTC_INDUCT
+  >> rpt strip_tac
+  >- simp[]
+  >> fs[reduction_def]
+  >> imp_res_tac choice_free_trans_pres
+  >> first_x_assum drule >> strip_tac
+  >> fs[GSYM reduction_def]
+  >> drule compile_network_preservation_trans >> simp[Once CONJ_SYM]
+  >> rpt(disch_then drule) >> strip_tac >> metis_tac[RTC_RTC]
+QED
+
+val _ = export_theory ();
